theories/soundness.v
@@ -1,0 +1,38 @@
+From Wasm Require Export type_preservation type_progress.
+From mathcomp Require Import ssreflect ssrbool eqtype.
+
+Set Implicit Arguments.
+Unset Strict Implicit.
+Unset Printing Implicit Defensive.
+
+Section Host.
+
+Context `{ho: host}.
+
+(* The same host function well-formedness assumptions from the interpreter *)
+Variable host_application_impl : host_state -> store_record -> function_type -> host_function -> list value -> (host_state * option (store_record * result)).
+
+Hypothesis host_application_impl_correct :
+  (forall hs s ft hf vs hs' hres, (host_application_impl hs s ft hf vs = (hs', hres)) -> host_application hs s ft hf vs hs' hres).
+
+CoInductive sound_trace hs s f es ts (Htype: config_typing s (f, es) ts) : Type :=
+| rt_terminal :
+  terminal_form es ->
+  sound_trace hs Htype
+| rt_step hs' s' f' es' (Htype': config_typing s' (f', es') ts):
+  reduce_tuple (hs, s, f, es) (hs', s', f', es') ->
+  sound_trace hs' Htype' ->
+  sound_trace hs Htype
+.
+
+CoFixpoint type_soundness hs s f es ts Htype: @sound_trace hs s f es ts Htype.
+Proof.
+  intros.
+  destruct (t_progress_interp_ctx host_application_impl_correct hs Htype) as [Hterm | [hs' [s' [f' [es' Hreduce]]]]] eqn:Hprogress.
+  - by apply rt_terminal.
+  - eapply rt_step.
+    + by apply Hreduce.
+    + by refine (type_soundness hs' _ _ _ _ (t_preservation Hreduce Htype)).
+Defined.
+    
+End Host.
